not working, just to same the progress, cub

code/experimental/P256/Hacl.Impl.P256.fst
@@ -776,62 +776,139 @@ let point_add_if_second_branch_impl result p q u1 u2 s1 s2 r h uh hCube tempBuff
   lemma_multiplication_not_mod_prime (as_nat h0 qZ) (modp_inv2 (pow2 256));
   lemmaFromDomain (as_nat h0 pZ);
   lemmaFromDomain (as_nat h0 qZ)
-    
- 
-#reset-options "--z3rlimit 200"
+
+
+val point_add: p: point -> q: point -> result: point -> tempBuffer: lbuffer uint64 (size 88) -> 
+   Stack unit (requires fun h -> live h p /\ live h q /\ live h result /\ live h tempBuffer /\ 
+   eq_or_disjoint q result /\
+   disjoint p q /\ disjoint p tempBuffer /\ disjoint q tempBuffer /\ disjoint p result /\ disjoint result tempBuffer /\  
+    as_nat h (gsub p (size 8) (size 4)) < prime /\ 
+    as_nat h (gsub p (size 0) (size 4)) < prime /\ 
+    as_nat h (gsub p (size 4) (size 4)) < prime /\
+    as_nat h (gsub q (size 8) (size 4)) < prime /\ 
+    as_nat h (gsub q (size 0) (size 4)) < prime /\  
+    as_nat h (gsub q (size 4) (size 4)) < prime 
+    ) 
+   (ensures fun h0 _ h1 -> 
+     modifies (loc tempBuffer |+| loc result) h0 h1 /\ 
+     as_nat h1 (gsub result (size 8) (size 4)) < prime /\ 
+     as_nat h1 (gsub result (size 0) (size 4)) < prime /\ 
+     as_nat h1 (gsub result (size 4) (size 4)) < prime /\
+     (
+       let pX, pY, pZ = gsub p (size 0) (size 4), gsub p (size 4) (size 4), gsub p (size 8) (size 4) in 
+       let qX, qY, qZ = gsub q (size 0) (size 4), gsub q (size 4) (size 4), gsub q (size 8) (size 4) in 
+       let x3, y3, z3 = gsub result (size 0) (size 4), gsub result (size 4) (size 4), gsub result (size 8) (size 4) in 
+       
+       let pxD, pyD, pzD = fromDomain_ (as_nat h0 pX), fromDomain_ (as_nat h0 pY), fromDomain_ (as_nat h0 pZ) in 
+       let qxD, qyD, qzD = fromDomain_ (as_nat h0 qX), fromDomain_ (as_nat h0 qY), fromDomain_ (as_nat h0 qZ) in 
+       let x3D, y3D, z3D = fromDomain_ (as_nat h1 x3), fromDomain_ (as_nat h1 y3), fromDomain_ (as_nat h1 z3) in
+      
+       let xN, yN, zN = _point_add (pxD, pyD, pzD) (qxD, qyD, qzD) in 
+       x3D == xN /\ y3D == yN /\ z3D == zN
+  )
+)
 
 let point_add p q result tempBuffer = 
     let h0 = ST.get() in 
-    
-   let z1 = sub p (size 8) (size 4) in 
-   let z2 = sub q (size 8) (size 4) in 
+  
+  let z1 = sub p (size 8) (size 4) in 
+  let z2 = sub q (size 8) (size 4) in 
 
-   let tempBuffer16 = sub tempBuffer (size 0) (size 16) in 
+  let tempBuffer16 = sub tempBuffer (size 0) (size 16) in 
    
-   let u1 = sub tempBuffer (size 16) (size 4) in 
-   let u2 = sub tempBuffer (size 20) (size 4) in 
-   let s1 = sub tempBuffer (size 24) (size 4) in 
-   let s2 = sub tempBuffer (size 28) (size 4) in 
+  let u1 = sub tempBuffer (size 16) (size 4) in 
+  let u2 = sub tempBuffer (size 20) (size 4) in 
+  let s1 = sub tempBuffer (size 24) (size 4) in 
+  let s2 = sub tempBuffer (size 28) (size 4) in 
 
-   let h = sub tempBuffer (size 32) (size 4) in 
-   let r = sub tempBuffer (size 36) (size 4) in 
-   let uh = sub tempBuffer (size 40) (size 4) in 
+  let h = sub tempBuffer (size 32) (size 4) in 
+  let r = sub tempBuffer (size 36) (size 4) in 
+  let uh = sub tempBuffer (size 40) (size 4) in 
 
-   let hCube = sub tempBuffer (size 44) (size 4) in 
+  let hCube = sub tempBuffer (size 44) (size 4) in 
 
-   let x3_out = sub tempBuffer (size 48) (size 4) in 
-   let y3_out = sub tempBuffer (size 52) (size 4) in 
-   let z3_out = sub tempBuffer (size 56) (size 4) in 
+  let x3_out = sub tempBuffer (size 48) (size 4) in 
+  let y3_out = sub tempBuffer (size 52) (size 4) in 
+  let z3_out = sub tempBuffer (size 56) (size 4) in 
 
-   let tempBuffer28 = sub tempBuffer (size 60) (size 28) in 
+  let tempBuffer28 = sub tempBuffer (size 60) (size 28) in 
 
-   move_from_jacobian_coordinates u1 u2 s1 s2 p q tempBuffer16;
-   let flag = point_double_condition u1 u2 s1 s2 z1 z2 in 
+  move_from_jacobian_coordinates u1 u2 s1 s2 p q tempBuffer16;
+    let h1 = ST.get() in 
+    assert(      
+      let pX, pY, pZ = as_nat h0 (gsub p (size 0) (size 4)), as_nat h0 (gsub p (size 4) (size 4)), as_nat h0 (gsub p (size 8) (size 4)) in 
+      let qX, qY, qZ = as_nat h0 (gsub q (size 0) (size 4)), as_nat h0 (gsub q (size 4) (size 4)), as_nat h0 (gsub q (size 8) (size 4)) in 
+      
+      let pxD, pyD, pzD = fromDomain_ pX, fromDomain_ pY, fromDomain_ pZ in 
+      let qxD, qyD, qzD = fromDomain_ qX, fromDomain_ qY, fromDomain_ qZ in 
 
-   if flag then
-      begin
-	let h0_1 = ST.get() in 
-	assert(modifies1 tempBuffer h0 h0_1);
-	point_double p result tempBuffer;
-	let h0_2 = ST.get() in 
-	  assert(modifies2 tempBuffer result h0_1 h0_2);
-	  assert(modifies2 tempBuffer result h0 h0_2)
-	  (*assert(Lib.Sequence.equal (as_seq h0_2 result) (point_add_seq (as_seq h0 p) (as_seq h0 q))) *)
-     end	   
-   else
-     begin
-       let h1_1 = ST.get() in 
-	   assert(modifies1 tempBuffer h0 h1_1);
-	 compute_common_params_point_add h r uh hCube u1 u2 s1 s2 tempBuffer16;
-	   let h1_2 = ST.get() in 
-	   assert (modifies1 tempBuffer h1_1 h1_2);  
-	 point_add_if_second_branch_impl result p q u1 u2 s1 s2 r h uh hCube tempBuffer28; 
-	   let h1_3 = ST.get() in  
-	   assert(modifies2 tempBuffer result h1_2 h1_3)
-     end; 
-   let hend = ST.get() in   
-   assert(modifies2 tempBuffer result h0 hend) (*;
-   assert(Lib.Sequence.equal (as_seq hend result) (point_add_seq (as_seq h0 p) (as_seq h0 q))) *)
+      as_nat h1 u1 == toDomain_ (qzD * qzD * pxD % prime256) /\
+      as_nat h1 u2 == toDomain_ (pzD * pzD * qxD % prime256) /\
+      as_nat h1 s1 == toDomain_ (qzD * qzD * qzD * pyD % prime256) /\
+      as_nat h1 s2 == toDomain_ (pzD * pzD * pzD * qyD % prime256));
+
+  let flag = point_double_condition u1 u2 s1 s2 z1 z2 in 
+    let h2 = ST.get() in 
+  if flag then
+    begin
+      point_double p result tempBuffer
+    end	   
+  else
+    begin
+      compute_common_params_point_add h r uh hCube u1 u2 s1 s2 tempBuffer16;
+      point_add_if_second_branch_impl result p q u1 u2 s1 s2 r h uh hCube tempBuffer28
+      
+    end; 
+
+  let h3 = ST.get() in 
+
+
+      let x1 = as_nat h0 (gsub p (size 0) (size 4)) in 
+      let y1 = as_nat h0 (gsub p (size 4) (size 4)) in 
+      let z1 = as_nat h0 (gsub p (size 8) (size 4)) in 
+
+      let x2 = as_nat h0 (gsub q (size 0) (size 4)) in 
+      let y2 = as_nat h0 (gsub q (size 4) (size 4)) in 
+      let z2 = as_nat h0 (gsub q (size 8) (size 4)) in 
+
+      let x3 = as_nat h3 (gsub result (size 0) (size 4)) in 
+      let y3 = as_nat h3 (gsub result (size 4) (size 4)) in 
+      let z3 = as_nat h3 (gsub result (size 8) (size 4)) in 
+
+      lemma_xToSpecification_ 
+	(fromDomain_ x1) (fromDomain_ y1) (fromDomain_ z1) (fromDomain_ x2) (fromDomain_ y2) (fromDomain_ z2) 
+	(as_nat h2 u1) (as_nat h2 u2) (as_nat h2 s1) (as_nat h2 s2) x3 y3 z3;
+
+    assert(    
+    
+    let (xN, yN, zN) = _point_add (fromDomain_ x1, fromDomain_ y1, fromDomain_ z1) 
+      (fromDomain_ x2, fromDomain_ y2, fromDomain_ z2) in
+    
+    let x3D, y3D, z3D = fromDomainPoint (x3, y3, z3) in 
+    let u1D = fromDomain_ (as_nat h2 u1) in let u2D = fromDomain_ (as_nat h2 u2) in 
+    let s1D = fromDomain_ (as_nat h2 s1) in let s2D = fromDomain_ (as_nat h2 s2) in 
+    (u1D = u2D && s1D = s2D && fromDomain_ z1 <> 0 && fromDomain_ z2 <> 0)  ==> (xN == x3D /\ yN == y3D /\ zN == z3D));
+
+     
+     assume(    
+    
+    let (xN, yN, zN) = _point_add (fromDomain_ x1, fromDomain_ y1, fromDomain_ z1) 
+      (fromDomain_ x2, fromDomain_ y2, fromDomain_ z2) in
+    
+    let x3D, y3D, z3D = fromDomainPoint (x3, y3, z3) in 
+    let u1D = fromDomain_ (as_nat h2 u1) in let u2D = fromDomain_ (as_nat h2 u2) in 
+    let s1D = fromDomain_ (as_nat h2 s1) in let s2D = fromDomain_ (as_nat h2 s2) in 
+    not(u1D = u2D && s1D = s2D && fromDomain_ z1 <> 0 && fromDomain_ z2 <> 0)  ==> (xN == x3D /\ yN == y3D /\ zN == z3D));
+
+
+    assert(    
+    
+    let (xN, yN, zN) = _point_add (fromDomain_ x1, fromDomain_ y1, fromDomain_ z1)  (fromDomain_ x2, fromDomain_ y2, fromDomain_ z2) in
+    
+    let x3D, y3D, z3D = fromDomainPoint (x3, y3, z3) in 
+    (xN == x3D /\ yN == y3D /\ zN == z3D))
+
+
 
 
 val lemma_pointAtInfInDomain: x: nat -> y: nat -> z: nat {z < prime256} -> 
