code/experimental/P256/Hacl.Spec.P256.MontgomeryMultiplication.PointAdd.fst
@@ -601,6 +601,71 @@ let point_add_if_second_branch_seq p q u1 u2 s1 s2 r h uh hCube =
 
 #reset-options "--z3rlimit 300"  
 
+
+val lemma_xToSpecification_ : 
+  x1D: nat -> y1D: nat -> z1D: nat -> x2D: nat -> y2D: nat -> z2D: nat -> 
+  
+  u1: nat{u1 = toDomain_ (z2D * z2D * x1D % prime)} -> 
+  u2: nat{u2 = toDomain_ (z1D * z1D * x2D % prime)} -> 
+  
+  s1: nat{s1 = toDomain_ (z2D * z2D * z2D * y1D % prime)} -> 
+  s2: nat{s2 = toDomain_ (z1D * z1D * z1D * y2D % prime)} ->
+
+  x3: nat{ 
+    let u1D, u2D = fromDomain_ u1, fromDomain_ u2 in 
+    let s1D, s2D = fromDomain_ s1, fromDomain_ s2 in  
+    (u1D = u2D && s1D = s2D && z1D <> 0 && z2D <> 0) ==> 
+      (let (xN, yN, zN) = _point_double (x1D, y1D, z1D) in fromDomain_ x3 == xN)} -> 
+   y3: nat{
+    let u1D, u2D = fromDomain_ u1, fromDomain_ u2 in 
+    let s1D, s2D = fromDomain_ s1, fromDomain_ s2 in  
+    (u1D = u2D && s1D = s2D && z1D <> 0 && z2D <> 0) ==> 
+      (let (xN, yN, zN) = _point_double (x1D, y1D, z1D) in fromDomain_ y3 == yN)} ->
+   z3: nat{
+     let u1D, u2D = fromDomain_ u1, fromDomain_ u2 in 
+     let s1D, s2D = fromDomain_ s1, fromDomain_ s2 in  
+     (u1D = u2D && s1D = s2D && z1D <> 0 && z2D <> 0) ==>
+       (let (xN, yN, zN) = _point_double (x1D, y1D, z1D) in fromDomain_ z3 == zN)}
+  ->  
+  Lemma 
+  (    
+    let (xN, yN, zN) = _point_add (x1D, y1D, z1D) (x2D, y2D, z2D) in
+    let x3D, y3D, z3D = fromDomainPoint (x3,  y3,  z3) in 
+    let u1D = fromDomain_ u1 in let u2D = fromDomain_ u2 in 
+    let s1D = fromDomain_ s1 in let s2D = fromDomain_ s2 in 
+    (u1D = u2D && s1D = s2D && z1D <> 0 && z2D <> 0)  ==> (xN == x3D /\ yN == y3D /\ zN == z3D)
+  )
+
+
+let lemma_xToSpecification_ x1D y1D z1D x2D y2D z2D u1 u2 s1 s2  x3 y3 z3 = 
+    let open FStar.Tactics in 
+    let open FStar.Tactics.Canon in 
+    let u1D = fromDomain_ u1 in let u2D = fromDomain_ u2 in 
+    let s1D = fromDomain_ s1 in let s2D = fromDomain_ s2 in  
+    
+    let (xN, yN, zN) = _point_add (x1D, y1D, z1D) (x2D, y2D, z2D) in 
+    let (xDouble, yDouble, zDouble) = _point_double (x1D, y1D, z1D) in 
+
+    let u1N = x1D * z2D * z2D % prime in 
+    let u2N = x2D * z1D * z1D % prime in 
+    let s1N = y1D * z2D * z2D * z2D % prime in 
+    let s2N = y2D * z1D * z1D * z1D % prime in 
+
+    assert_by_tactic (x1D * z2D * z2D = x1D * (z2D * z2D)) canon;
+    assert_by_tactic (x2D * z1D * z1D = x2D * (z1D * z1D)) canon;
+    
+    assert_by_tactic (y1D * z2D * (z2D * z2D) = y1D * z2D * z2D * z2D) canon;
+    assert_by_tactic (y2D * z1D * (z1D * z1D) = y2D * z1D * z1D * z1D) canon;
+
+
+     lemmaToDomainAndBackIsTheSame (u1N);
+     lemmaToDomainAndBackIsTheSame (u2N);
+     lemmaToDomainAndBackIsTheSame (s1N);
+     lemmaToDomainAndBackIsTheSame (s2N)
+     
+
+
+
  
 val lemma_xToSpecification : x1D: nat -> y1D: nat -> z1D: nat -> x2D: nat -> y2D: nat -> z2D: nat -> 
   u1: felem_seq_prime{fromDomain_(felem_seq_as_nat u1) = x1D * z2D * z2D % prime} -> 
@@ -660,6 +725,88 @@ let lemma_xToSpecification x1D y1D z1D x2D y2D z2D u1 u2 s1 s2  x3 y3 z3 =
      lemmaFromDomainToDomain (felem_seq_as_nat x3);
      lemmaFromDomainToDomain (felem_seq_as_nat y3);
      lemmaFromDomainToDomain (felem_seq_as_nat z3)
+
+
+
+
+
+
+
+
+
+
+
+
+
+
+noextract       
+assume val lemma_xToSpecification_after_double_: 
+  pX: nat -> pY: nat -> pZ: nat -> 
+
+  qX: nat -> qY: nat -> qZ: nat -> 
+
+  x3: nat -> y3: nat -> z3: nat -> 
+  
+  u1: nat -> u2: nat -> s1: nat -> s2: nat -> h: nat -> r: nat -> 
+  Lemma
+    (requires (    
+
+      let pxD, pyD, pzD = fromDomain_ pX, fromDomain_ pY, fromDomain_ pZ in 
+      let qxD, qyD, qzD = fromDomain_ qX, fromDomain_ qY, fromDomain_ qZ in 
+      let x3D, y3D, z3D = fromDomain_ x3, fromDomain_ y3, fromDomain_ z3 in 
+
+      let u1D = fromDomain_ u1 in 
+      let u2D = fromDomain_ u2 in 
+      let s1D = fromDomain_ s1 in 
+      let s2D = fromDomain_ s2 in 
+
+      let rD = fromDomain_ r in 
+      let hD = fromDomain_ h in 
+     
+      u1 == toDomain_ (qzD * qzD * pxD % prime256) /\
+      u2 == toDomain_ (pzD * pzD * qxD % prime256) /\
+      s1 == toDomain_ (qzD * qzD * qzD * pyD % prime256) /\
+      s2 == toDomain_ (pzD * pzD * pzD * qyD % prime256) /\
+      
+      h == toDomain_ ((u2D - u1D) % prime256) /\
+      r == toDomain_ ((s2D - s1D) % prime256) /\
+
+      (
+	if (not (fromDomain_ u1 = fromDomain_ u2 && fromDomain_ s1 = fromDomain_ s2 && pzD <> 0 && qzD <> 0)) then 
+	(
+	  if qzD = 0 then 
+	    fromDomain_ x3 == pxD /\ 
+	    fromDomain_ y3 == pyD /\ 
+	    fromDomain_ z3 == pzD
+	  else if pzD = 0 then 
+	    fromDomain_ x3 == qxD /\ 
+	    fromDomain_ y3 == qyD /\ 
+	    fromDomain_ z3 == qzD 
+	  else
+	    begin
+	      fromDomain_ x3 == (rD * rD - hD * hD * hD - 2 * u1D * hD * hD) % prime /\
+	      fromDomain_ y3 == (rD * (u1D * hD * hD - x3D) - s1D * hD*hD*hD) % prime /\
+	      fromDomain_ z3 == (hD * pzD * qzD) % prime
+	    end
+	)
+	else True)
+  )
+)
+  (ensures 
+  (    
+      let pxD, pyD, pzD = fromDomain_ pX, fromDomain_ pY, fromDomain_ pZ in 
+      let qxD, qyD, qzD = fromDomain_ qX, fromDomain_ qY, fromDomain_ qZ in 
+      let x3D, y3D, z3D = fromDomain_ x3, fromDomain_ y3, fromDomain_ z3 in 
+
+     let (xN, yN, zN) = _point_add (pxD, pyD, pzD) (qxD, qyD, qzD) in
+     
+     let u1D = fromDomain_ u1 in let u2D = fromDomain_ u2 in 
+     let s1D = fromDomain_ s1 in let s2D = fromDomain_ s2 in 
+     if (not(u1D = u2D && s1D = s2D && pzD <> 0 && qzD <> 0)) then
+       xN == x3D /\  yN == y3D /\ zN == z3D
+     else True
+  )
+)
 
 
 noextract       
